\appendix
\section{Symbols and their meanings}
\printunsrtglossary[type=symbols,style=long]

\section{Gaussian distribution}
\subsection{Converting probability to its log-probability}\label{AP:log_prob}
\begin{equation}\label{eq:ap_logprob}
\begin{split}
    \ln p(\textbf{x}^n_1 | \mu, \sigma^2) &= \prod_{i=1}^{n}{\mathcal{N}(x_i|\mu, \sigma^2)}\\
    \ln p(\textbf{x}^n_1 | \mu, \sigma^2) &= \ln \prod_{i=1}^{n}\frac{1}{(2 \pi \sigma ^2)^{\frac{1}{2}}} e^{- \frac{1}{2\sigma ^2}(x_i - \mu)^2}\\
    \ln p(\textbf{x}^n_1 | \mu, \sigma^2) &= \sum_{i=1}^{n} \ln \frac{1}{(2 \pi \sigma ^2)^{\frac{1}{2}}} e^{- \frac{1}{2\sigma ^2}(x_i - \mu)^2}\\
    \ln p(\textbf{x}^n_1 | \mu, \sigma^2) &= \sum_{i=1}^{n} \ln \frac{1}{(2 \pi \sigma ^2)^{\frac{1}{2}}} + \ln e^{- \frac{1}{2\sigma ^2}(x_i - \mu)^2}\\
    \ln p(\textbf{x}^n_1 | \mu, \sigma^2) &= \sum_{i=1}^{n} -\frac{1}{2} \ln (2 \pi \sigma ^2) - \frac{1}{2\sigma ^2}(x_i - \mu)^2\\
    \ln p(\textbf{x}^n_1 | \mu, \sigma^2) &= \sum_{i=1}^{n} -\frac{1}{2} \ln (2 \pi \sigma ^2) - \frac{1}{2\sigma ^2}(x_i - \mu)^2\\
    \ln p(\textbf{x}^n_1 | \mu, \sigma^2) &= -\frac{n}{2} \ln 2 \pi -\frac{n}{2} \ln \sigma ^2 - \sum_{i=1}^{n} \frac{1}{2\sigma ^2}(x_i - \mu)^2\\
\end{split}
\end{equation}

\subsection{Maximum likelihood for $\mu$}\label{AP:mu_ML}
\begin{equation}\label{eq:ap_derivative_mu}
\begin{split}
    \frac{\partial }{\partial \mu } \big( - \frac{n}{2} \ln{2 \pi} - \frac{n}{2} \ln{\sigma ^2} - \sum_{i=1}^{n} \frac{1}{2\sigma ^2}(x_i - \mu_{ML})^2 \big) &= 0\\
    \frac{\partial}{\partial \mu} \big( - \sum_{i=1}^{n} \frac{1}{2\sigma ^2}(x_i - \mu_{ML})^2 \big) &= 0\\
    - \sum_{i=1}^{n} \frac{1}{2\sigma ^2}(-2 x_i + 2 \mu_{ML}) &= 0\\
    \sum_{i=1}^{n} \frac{2 x_i}{2\sigma ^2} &= \sum_{i=1}^{n} \frac{2 \mu_{ML}}{2\sigma ^2}\\
    \sum_{i=1}^{n} x_i &= n \mu_{ML}\\
    \frac{1}{n} \sum_{i=1}^{n} x_i &= \mu_{ML}\\
\end{split}
\end{equation}

\subsection{Maximum likelihood for $\sigma^2$}\label{AP:s2_ML}

\begin{equation}\label{eq:ap_derivative_sigma}
\begin{split}
    \frac{\partial }{\partial \sigma^2 } \big( - \frac{n}{2} \ln{2 \pi} - \frac{n}{2} \ln{\sigma^2_{ML}} - \sum_{i=1}^{n} \frac{1}{2\sigma^2_{ML}}(x_i - \mu_{ML})^2 \big) &= 0\\
    \frac{\partial}{\partial \sigma^2} \big( - \frac{n}{2} \ln{\sigma^2_{ML}}  - \sum_{i=1}^{n} \frac{1}{2\sigma^2_{ML}}(x_i - \mu_{ML})^2 \big) &= 0\\
    \frac{n}{2\sigma^2_{ML}} - \sum_{i=1}^{n} \frac{1}{2{\sigma^2_{ML}}^2}(x_i - \mu_{ML})^2 &= 0\\
    n\sigma^2_{ML} - \sum_{i=1}^{n} (x_i - \mu_{ML})^2 &= 0\\
    \frac{1}{n} \sum_{i=1}^{n} (x_i - \mu_{ML})^2 &= \sigma^2_{ML}\\
\end{split}
\end{equation}
